checkpoint

src/add_multiply.v
@@ -9,6 +9,8 @@ Inductive Instr :=
 | Mul (rd rs1 rs2 : Bit 5)
 | Unknown.
 
+Instance defaultInstr : Default Instr := Unknown.
+
 Inductive method :=
 | GetIReq
 | GetIResp (resp : Instr)
@@ -19,196 +21,203 @@ Inductive state :=
 | State__Decode
 | State__Execute.
 
-Inductive implLeakage :=
-| ImplLeak__GetIReq
-| ImplLeak__GetIResp
-| ImplLeak__Rule.
+Inductive implLeak :=
+| ImplLeak__Pc (l : Bit 32)
+| ImplLeak__Add
+| ImplLeak__Mul (a : Bit 4).
 
 Instance state__EqDecision : EqDecision state.
 Proof.
   solve_decision.
 Defined.
 
-Module AddMultiply.
-  Inductive D2E :=
-  | DAdd (rd : Bit 5) (v1 v2 : Bit 4)
-  | DMul (rd : Bit 5) (v1 v2 : Bit 4).
+Inductive D2E :=
+| DAdd (rd : Bit 5) (v1 v2 : Bit 4)
+| DMul (rd : Bit 5) (v1 v2 : Bit 4).
 
-  Record t :=
-    { m : Multiplier.t
-    ; rf : RegFile.t 4 5
-    ; pc : Bit 32
-    ; fromImem : Fifo.t Instr
-    ; toImem : Fifo.t (Bit 32)
-    ; d2e : Fifo.t D2E
-    ; st : state
-    ; trace : list implLeakage
-    }.
+Instance defaultD2E : Default D2E := DAdd 0%bv 0%bv 0%bv.
 
-  Definition mk :=
-    {| m := Multiplier.mk
-    ; rf := RegFile.mk
-    ; pc := 0%bv
-    ; fromImem := Fifo.mk
-    ; toImem := Fifo.mk
-    ; d2e := Fifo.mk
-    ; st := State__Fetch
-    ; trace := []
-    |}.
+Record AddMultiply :=
+  { addMultiplyM : Multiplier
+  ; addMultiplyRf : RegFile 4 5
+  ; addMultiplyPc : Bit 32
+  ; addMultiplyFromImem : Fifo Instr
+  ; addMultiplyToImem : Fifo (Bit 32)
+  ; addMultiplyD2E : Fifo D2E
+  ; addMultiplySt : state
+  ; addMultiplyTrace : list implLeak
+  }.
 
-  Definition getIReq :=
-    {{ let%read toImem0 := toImem in
-       if (Fifo.notEmpty toImem0) then
-         let%modify trace := snoc ImplLeak__GetIReq in
-         let%call d := Fifo.deq on toImem in
-         match d with
-         | Valid d => ret d
-         | Invalid => ret 0%bv
-         end
-       else
-         ret 0%bv
-    }}.
+Definition mkAddMultiply :=
+  {|
+    addMultiplyM := mkMultiplier;
+    addMultiplyRf := mkRegFile;
+    addMultiplyPc := 0%bv;
+    addMultiplyFromImem := mkFifo;
+    addMultiplyToImem := mkFifo;
+    addMultiplyD2E := mkFifo;
+    addMultiplySt := State__Fetch;
+    addMultiplyTrace := []
+  |}.
 
-  Definition getIResp instr :=
-    {{ let%read fromImem0 := fromImem in
-       let%read toImem0 := toImem in
-       guard (Fifo.notFull fromImem0 && Fifo.notFull toImem0) then
-         let%modify trace := snoc ImplLeak__GetIResp in
-         let%call _ := Fifo.enq instr on fromImem in
-         pass
-    }}.
+Definition addMultiplyGetIReq :=
+  {{ let%read toImem := addMultiplyToImem in
+     if fifoNotEmpty toImem then
+       let%call d := fifoDeq on addMultiplyToImem in
+       ret d
+     else
+       ret 0%bv
+  }}.
 
-  Definition fetch :=
-    {{ let%read pc0 := pc in
-       let%read toImem0 := toImem in
-       guard (Fifo.notFull toImem0) then
-         let%modify trace := snoc ImplLeak__Rule in
-         let%call _ := Fifo.enq pc0 on toImem in
-         let%write st := State__Decode in
-         pass
-    }}.
-
-  Definition decode :=
-    {{ let%read fromImem0 := fromImem in
-       let%read toImem0   := toImem in
-       let%read d2e0      := d2e in
-       let%read rf0       := rf in
-       guard (Fifo.notFull d2e0 && Fifo.notEmpty fromImem0 && Fifo.notFull toImem0) then
-         let%modify trace := snoc ImplLeak__Rule in
-         let%call instr := Fifo.deq on fromImem in
-         match instr with
-         | Valid Unknown =>
-             let%write st := State__Fetch in pass
-         | Valid (Add rd rs1 rs2) =>
-             let v1 := RegFile.sub rs1 rf0 in
-             let v2 := RegFile.sub rs2 rf0 in
-             let%call _ := Fifo.enq (DAdd rd v1 v2) on d2e in
-             let%write st := State__Execute in
-             pass
-         | Valid (Mul rd rs1 rs2) =>
-             let v1 := RegFile.sub rs1 rf0 in
-             let v2 := RegFile.sub rs2 rf0 in
-             let%call _ := Fifo.enq (DMul rd v1 v2) on d2e in
-             let%write st := State__Execute in
-             pass
-         | Valid (Addi rd rs1 imm) =>
-             let v1 := RegFile.sub rs1 rf0 in
-             let%call _ := Fifo.enq (DAdd rd v1 imm) on d2e in
-             let%write st := State__Execute in
-             pass
-         | Invalid => pass
-         end
-    }}.
-
-  Definition executeAdd rd v1 v2 :=
-    {{ let%call _ := Fifo.deq on d2e in
-       let%call _ := RegFile.upd rd (v1 + v2)%bv on rf in
-       let%write st := State__Fetch in
-       let%modify pc := fun pc => (pc `+Z` 4)%bv in
+Definition addMultiplyGetIResp instr :=
+  {{ let%read fromImem := addMultiplyFromImem in
+     let%read toImem := addMultiplyToImem in
+     when fifoNotFull fromImem && fifoNotFull toImem then
+       let%call _ := fifoEnq instr on addMultiplyFromImem in
        pass
-    }}.
+  }}.
 
-  Definition executeMul rd v1 v2 :=
-    {{ let%read m0 := m in
-       match Multiplier.st m0 with
-       | State__Empty =>
-           let%call _ := Multiplier.enq v1 v2 on m in
+Definition addMultiplyFetch :=
+  {{ let%read pc := addMultiplyPc in
+     let%read toImem := addMultiplyToImem in
+     when fifoNotFull toImem then
+       let%call _ := fifoEnq pc on addMultiplyToImem in
+       let%write addMultiplySt := State__Decode in
+       pass
+  }}.
+
+Definition addMultiplyDecode :=
+  {{ let%read fromImem := addMultiplyFromImem in
+     let%read toImem   := addMultiplyToImem in
+     let%read d2e      := addMultiplyD2E in
+     let%read rf       := addMultiplyRf in
+     when fifoNotFull d2e && fifoNotEmpty fromImem && fifoNotFull toImem then
+       let%call instr := fifoDeq on addMultiplyFromImem in
+       match instr with
+       | Unknown =>
+           (* In this case, an unknown instruction is encounteted, could
+              just send a no-op to the execution unit instead. *)
+           let%write addMultiplySt := State__Fetch in pass
+       | Add rd rs1 rs2 =>
+           let v1 := regFileSub rs1 rf in
+           let v2 := regFileSub rs2 rf in
+           let%call _ := fifoEnq (DAdd rd v1 v2) on addMultiplyD2E in
+           let%write addMultiplySt := State__Execute in
            pass
-       | State__Busy =>
-           let%call _ := Multiplier.rule on m in
+       | Mul rd rs1 rs2 =>
+           let v1 := regFileSub rs1 rf in
+           let v2 := regFileSub rs2 rf in
+           let%call _ := fifoEnq (DMul rd v1 v2) on addMultiplyD2E in
+           let%write addMultiplySt := State__Execute in
            pass
-       | State__Full =>
-           let%call v := Multiplier.deq on m in
-           match v with
-           | Valid v =>
-               let%call _ := Fifo.deq on d2e in
-               let%call _ := RegFile.upd rd (truncate v) on rf in
-               let%write st := State__Fetch in
-               let%modify pc := fun pc => (pc `+Z` 4)%bv in
-               pass
-           | Invalid => pass
-           end
+       | Addi rd rs1 imm =>
+           let v1 := regFileSub rs1 rf in
+           let%call _ := fifoEnq (DAdd rd v1 imm) on addMultiplyD2E in
+           let%write addMultiplySt := State__Execute in
+           pass
        end
-    }}.
+  }}.
 
-  Definition execute :=
-    {{ let%read d2e0 := d2e in
-       guard (Fifo.notEmpty d2e0) then
-         let%modify trace := snoc ImplLeak__Rule in
-         let instr := Fifo.first d2e0 in
-         match instr with
-         | Valid (DAdd rd v1 v2) => executeAdd rd v1 v2
-         | Valid (DMul rd v1 v2) => executeMul rd v1 v2
+Definition addMultiplyExecuteAdd rd v1 v2 :=
+  {{ let%read pc := addMultiplyPc in
+     let%call _ := fifoDeq on addMultiplyD2E in
+     let%call _ := regFileUpd rd (v1 + v2)%bv on addMultiplyRf in
+     let%write addMultiplySt := State__Fetch in
+     let%modify addMultiplyTrace := snoc (ImplLeak__Pc pc) in
+     let%modify addMultiplyTrace := snoc ImplLeak__Add in
+     let%modify addMultiplyPc := fun pc => (pc `+Z` 4)%bv in
+     pass
+  }}.
+
+Definition addMultiplyExecuteMul rd v1 v2 :=
+  {{ let%read m := addMultiplyM in
+     let%read pc := addMultiplyPc in
+     match m.(multiplierSt) with
+     | State__Empty =>
+         let%call _ := multiplierEnq v1 v2 on addMultiplyM in
+         pass
+     | State__Busy =>
+         let%call _ := multiplierRule on addMultiplyM in
+         pass
+     | State__Full =>
+         let%call v := multiplierDeq on addMultiplyM in
+         match v with
+         | Valid v =>
+             let%call _ := fifoDeq on addMultiplyD2E in
+             let%call _ := regFileUpd rd (truncate v) on addMultiplyRf in
+             let%write addMultiplySt := State__Fetch in
+             let%modify addMultiplyTrace := snoc (ImplLeak__Pc pc) in
+             let%modify addMultiplyTrace := snoc (ImplLeak__Mul v1) in
+             let%modify addMultiplyPc := fun pc => (pc `+Z` 4)%bv in
+             pass
          | Invalid => pass
          end
-    }}.
+     end
+  }}.
 
-  Definition rule :=
-    {{ let%read st0 := st in
-       match st0 with
-       | State__Fetch => fetch
-       | State__Decode => decode
-       | State__Execute => execute
+Definition addMultiplyExecute :=
+  {{ let%read d2e := addMultiplyD2E in
+     when fifoNotEmpty d2e then
+       let instr := fifoFirst d2e in
+       match instr with
+       | DAdd rd v1 v2 => addMultiplyExecuteAdd rd v1 v2
+       | DMul rd v1 v2 => addMultiplyExecuteMul rd v1 v2
        end
-    }}.
+  }}.
 
-  Instance circuit : Circuit :=
-    {| circuitInit := mk
-    ; circuitResult m :=
-        match m with
-        | GetIReq => Bit 32
-        | GetIResp _ => unit
-        | Rule => unit
-        end
-    ; circuitCall m :=
-        match m with
-        | GetIReq => getIReq
-        | GetIResp resp => getIResp resp
-        | Rule => rule
-        end
-    ; circuitTrace := trace
-    |}.
-End AddMultiply.
+Definition addMultiplyRule :=
+  {{ let%read st := addMultiplySt in
+     match st with
+     | State__Fetch => addMultiplyFetch
+     | State__Decode => addMultiplyDecode
+     | State__Execute => addMultiplyExecute
+     end
+  }}.
+
+Instance addMultiplyCircuit : Circuit :=
+  {| circuitInit := mkAddMultiply
+  ; circuitResult m :=
+      match m with
+      | GetIReq => Bit 32
+      | _ => unit
+      end
+  ; circuitCall m :=
+      match m with
+      | GetIReq => addMultiplyGetIReq
+      | GetIResp resp => addMultiplyGetIResp resp
+      | Rule => addMultiplyRule
+      end
+  ; circuitTrace := addMultiplyTrace
+  |}.
 
 Section example.
-  Notation runCircuit := (runCircuit (c := AddMultiply.circuit)).
-
   Definition ms :=
-    [Rule (* fetch *)
+    [Rule
      ; GetIReq
      ; GetIResp (Addi 1%bv 0%bv 3%bv)
-     ; Rule (* decode *)
-     ; Rule (* execute *)
-     ; Rule (* fetch  *)
+     ; Rule
+     ; Rule
+     ; Rule
      ; GetIReq
      ; GetIResp (Addi 2%bv 0%bv 4%bv)
-     ; Rule (* decode *)
-     ; Rule (* execute *)
-     ; Rule (* fetch *)
+     ; Rule
+     ; Rule
+     ; Rule
      ; GetIReq
      ; GetIResp (Mul 3%bv 1%bv 2%bv)
-     ; Rule (* decode *)
-     ; Rule (* execute... *)
+     ; Rule
+     ; Rule
+     ; Rule
+     ; Rule
+     ; Rule
+     ; Rule
+     ; Rule
+     ; Rule
+     ; Rule
+     ; GetIReq
+     ; GetIResp (Mul 4%bv 3%bv 2%bv)
+     ; Rule
+     ; Rule
      ; Rule
      ; Rule
      ; Rule
@@ -217,5 +226,5 @@ Section example.
      ; Rule
     ].
 
-  Eval vm_compute in runCircuit ms.
+  Eval vm_compute in runCircuit addMultiplyCircuit ms.
 End example.
