src/regfile.v
@@ -1,27 +1,21 @@
 From research Require Import base bit circuit.
 From stdpp Require Import fin finite vector.
 
-Module RegFile.
-  Section WithContext.
-    Context (b : N) (sz : N) {H0 : BvWf b 0} {H1 : BvWf sz 0}.
+Section WithContext.
+  Context (b : N) (sz : N).
 
-    Record t := { contents : Vector (Bit b) (card (Bit sz)) }.
+  Record RegFile := { regFileContents : Vector (Bit b) (card (Bit sz)) }.
 
-    Definition mk := {| contents := mkVector 0%bv (card (Bit sz)) |}.
+  Definition mkRegFile := {| regFileContents := mkVector δ (card (Bit sz)) |}.
 
-    Definition sub (addr : Bit sz) (t : t) :=
-      if decide (addr = 0)%bv then
-        0%bv
-      else
-        t.(contents) !!! encode_fin addr.
+  Definition regFileSub (addr : Bit sz) (t : RegFile) :=
+    if decide (addr = δ)%bv then δ else t.(regFileContents) !!! encode_fin addr.
 
-    Definition upd (addr : Bit sz) (data : Bit b) :=
-      {{ let%modify contents := vinsert (encode_fin addr) data in
-         pass
-      }}.
-  End WithContext.
+  Definition regFileUpd (addr : Bit sz) (data : Bit b) :=
+    {{ let%modify regFileContents := vinsert (encode_fin addr) data in
+       pass
+    }}.
+End WithContext.
 
-  Arguments mk {_ _ _}.
-  Arguments sub {_ _ _ _}.
-  Arguments upd {_ _}.
-End RegFile.
+Arguments mkRegFile {_ _}.
+Arguments regFileSub {_ _}.
